src/test/scala/qrhl/tactic/ExpressionTest.scala
@@ -2,6 +2,7 @@ package qrhl.tactic
 
 import org.scalatest.FunSuite
 import qrhl.isabelle.Isabelle
+import qrhl.logic.Expression
 import qrhl.toplevel.ToplevelTest
 
 class ExpressionTest extends FunSuite {
@@ -14,5 +15,39 @@ class ExpressionTest extends FunSuite {
     println(e)
     println(t)
     assert(state.isabelle.checkType(t) == Isabelle.expressionT(Isabelle.predicateT))
+  }
+
+  test("encodeAsExpression roundtrip") {
+    val tl = ToplevelTest.makeToplevel()
+    tl.execCmd("classical var x : int")
+    val state = tl.state
+    val e = state.parseExpression(Isabelle.predicateT,"Cla[ x=(1::int) ]")
+    println(e)
+    val t = e.encodeAsExpression(tl.state.isabelle)
+    println(Isabelle.pretty(t))
+    val e2 = Expression.decodeFromExpression(tl.state.isabelle, t)
+    println(e2)
+
+    assert(e.isabelleTerm==e2.isabelleTerm)
+    assert(e.typ==e2.typ)
+    assert(e==e2)
+
+  }
+
+  test("encodeAsExpression roundtrip 2") {
+    val tl = ToplevelTest.makeToplevel()
+    tl.execCmd("classical var x : int")
+    val state = tl.state
+    val e = state.parseExpression(Isabelle.predicateT,"Cla[ x1=x2 ]")
+    println(e)
+    val t = e.encodeAsExpression(tl.state.isabelle)
+    println(Isabelle.pretty(t))
+    val e2 = Expression.decodeFromExpression(tl.state.isabelle, t)
+    println(e2)
+
+    assert(e.isabelleTerm==e2.isabelleTerm)
+    assert(e.typ==e2.typ)
+    assert(e==e2)
+
   }
 }
