src/test/scala/qrhl/tactic/SeqTacTest.scala
@@ -3,17 +3,21 @@ package qrhl.tactic
 import org.scalatest.FunSuite
 import qrhl.QRHLSubgoal
 import qrhl.isabelle.Isabelle
+import qrhl.logic.{Expression, Statement}
 import qrhl.toplevel.ToplevelTest
 
 class SeqTacTest extends FunSuite {
-  test("seq rule succeeds") {
+  def testSeqRule(pre:String,post:String,left:String,right:String,middle:String) : Unit = {
     val tl = ToplevelTest.makeToplevel()
     tl.execCmd("classical var x : int")
     val state = tl.state
-    val left = state.parseBlock("x <- 1; x <- 2;")
-    val pre = state.parseExpression(Isabelle.predicateT,"Cla[ x=(1::int) ]")
-    val qrhl = QRHLSubgoal(left,left,pre,pre,Nil)
-    val tac = SeqTac(1,1,state.parseExpression(Isabelle.predicateT,"Cla[False]"))
+    val left2 = state.parseBlock(left)
+    val right2 = state.parseBlock(right)
+    val pre2 = state.parseExpression(Isabelle.predicateT,pre)
+    val post2 = state.parseExpression(Isabelle.predicateT,post)
+    val qrhl = QRHLSubgoal(left2,right2,pre2,post2,Nil)
+    val middle2 = state.parseExpression(Isabelle.predicateT,middle)
+    val tac = SeqTac(1,1,middle2)
     val goals = tac(state,qrhl)
     assert(goals.length == 2)
     val List(goal1,goal2) = goals
@@ -21,5 +25,21 @@ class SeqTacTest extends FunSuite {
     goal2.checkWelltyped(tl.state.isabelle)
     assert(goal1.isInstanceOf[QRHLSubgoal])
     assert(goal2.isInstanceOf[QRHLSubgoal])
+    val qrhl1 = goal1.asInstanceOf[QRHLSubgoal]
+    val qrhl2 = goal2.asInstanceOf[QRHLSubgoal]
+    assert(qrhl1.pre == pre2)
+    assert(qrhl2.post == post2)
+    assert(qrhl1.post == middle2)
+    assert(qrhl2.pre == middle2)
+  }
+
+  test("seq rule succeeds") {
+    testSeqRule("Cla[ x=(1::int) ]", "Cla[ x=(1::int) ]",
+      "x <- 1; x <- 2;", "x <- 1; x <- 2;", "Cla[False]")
+  }
+
+  test("seq rule succeeds, x1=x2") {
+    testSeqRule("Cla[ x=(1::int) ]", "Cla[ x=(1::int) ]",
+      "x <- 1; x <- 2;", "x <- 1; x <- 2;", "Cla[x1=x2]")
   }
 }
