src/main/isabelle/Test.thy
@@ -2,69 +2,7 @@ theory Test
   imports Tactics
 begin
 
-
-ML {*
-*}
-
-ML {*
-*}
-
-ML {*
-*}
-
-
-ML {*
-*}
-
-(*ML {*
-  Outer_Syntax.command @{command_keyword variables2} "bla"
-  (Scan.succeed (Toplevel.open_target (fn gthy =>
-    let val lthy = Bundle.context [] [] gthy |> #2
-        val lthy2 = QRHL.declare_variable lthy @{binding "a"} @{typ bool} QRHL.Classical
-        val lthy3 = QRHL.declare_variable lthy2 @{binding "q"} @{typ nat} QRHL.Quantum
-  in lthy3 end
-  )))
-*}*)
-
-(* ML {*
-fun variables2 vars gthy =
-let val lthy = Bundle.context [] [] gthy |> #2
-    val lthy2 = fold (fn (cq,bind,T) => fn lthy' => QRHL.declare_variable lthy' bind T cq) vars lthy
-in lthy2 end
-*}
-
-ML {*
-fun variables2_cmd vars gthy = 
-  let val ctxt = Context.proof_of gthy
-      val vars' = map (fn (a,b,c) => (a,b,Syntax.read_typ ctxt c)) vars
-  in
-    variables2 vars' gthy
-  end
-*}
-
-ML {*
-val parse_classical_quantum = (Parse.reserved "classical" >> K QRHL.Classical) || (Parse.reserved "quantum" >> K QRHL.Quantum)
-val _ =
-  Outer_Syntax.command @{command_keyword variables2} "declare quantum/classical variables"
-    ((Parse.and_list (parse_classical_quantum -- Args.binding --| Parse.$$$ "::" -- Parse.typ >> (fn ((a,b),c) => (a,b,c))) >> 
-      (fn vars => Toplevel.open_target (variables2_cmd vars)))
-        --| Parse.begin)
-*}
- *)
-(* 
-variables2 classical a :: int and quantum q :: nat begin
-term a_var
-term a
-term q
-thm a_varname
-
-lemma l: "variable_name a_var = ''a''" by simp
-
-end
-
-lemma l: "variable_name a_var = ''a''" by simp
- *)
-
+(* TODO: to Encoding *)
 lemma tmp3[simp]: 
   fixes e :: "('a*'b)*'c \<Rightarrow> 'e"
   defines "f == (\<lambda>(a,b,c). e ((a,b),c))"
@@ -72,42 +10,12 @@ lemma tmp3[simp]:
     = expression (qvariable_concat S (qvariable_concat Q R)) f"
   sorry
 
+(* TODO: to Encoding *)
 lemma tmp4[simp]: 
   fixes e :: "'a*unit \<Rightarrow> 'e"
-  (* defines "f == (\<lambda>(a,b,c). e ((a,b),c))" *)
   shows "expression (qvariable_concat Q \<lbrakk>\<rbrakk>) e = expression Q (\<lambda>a. e (a,()))"
   sorry
 
-(* context begin
-
-lemma xxx[simp]: "1=2" sorry
-
-declare[[method_error]]
-
-local_setup {*
-decl_var_hack "x" @{typ int} QRHL.Classical
-*}
-
-lemma "1=1" by auto
-definition "q=1" 
-
-ML {*
-QRHL.VarTypes.get @{context} |> Symtab.dest
-*}
-
-end
-
-ML {*
-QRHL.VarTypes.get @{context} |> Symtab.dest
-*}
-
-lemma "1=2" by simp
-ML {* Config.get @{context} Tactics.method_error *}
-
-ML {* Config.get @{context} Tactics.method_error *}
-
-ML Config.declare
- *)
 
 variables
   classical x :: int and
@@ -116,45 +24,82 @@ variables
   classical c :: int
 begin
 
-
+(* TODO: generalize *)
 lemma tmp[simp]: "subst_expression (substitute1 v (const_expression z)) (expression \<lbrakk>v\<rbrakk> f)
 = const_expression (f z)" sorry
 
-lemma tmp2[simp]: "index_var True x_var = x1_var" sorry
+
+lemma qrhl_top: "qrhl A p1 p2 (expression Q (\<lambda>z. top))" sorry
+
+lemma index_var_conv_helper1:
+  assumes "variable_name v \<equiv> vname"
+  assumes "variable_name v1 \<equiv> v1name"
+  assumes "vname @ ''1'' \<equiv> v1name"
+  shows "index_var True v \<equiv> v1"
+  using assms index_var1I by smt
+
+lemma index_var_conv_helper2:
+  assumes "variable_name v \<equiv> vname"
+  assumes "variable_name v2 \<equiv> v2name"
+  assumes "vname @ ''2'' \<equiv> v2name"
+  shows "index_var False v \<equiv> v2"
+  using assms index_var2I by smt
+
+ML {*
+fun index_var_conv ctxt ct =
+  let val (lrname,x,T) = case Thm.term_of ct of
+        Const(@{const_name index_var},_) $ Const(lrname,_) $ Free(x,T) => (lrname,x,T)
+      | _ => raise CTERM("index_var_conv: wrong shape",[ct])
+      val lr = case lrname of 
+          @{const_name True} => true
+        | @{const_name False} => false
+        | _ => raise CTERM("index_var_conv: wrong shape (expected True/False as first arg)",[ct])
+
+      val suffix = (if lr then "1" else "2")
+      val x1 = x ^ suffix
+
+      val varname_x = Raw_Simplifier.rewrite_cterm (false,false,false) (fn _ => fn _ => NONE) ctxt (Thm.cterm_of ctxt 
+        (Const(@{const_name variable_name}, T --> @{typ string}) $ Free(x,T)))
+
+      val varname_x1 = Raw_Simplifier.rewrite_cterm (false,false,false) (fn _ => fn _ => NONE) ctxt (Thm.cterm_of ctxt 
+        (Const(@{const_name variable_name}, T --> @{typ string}) $ Free(x1,T)))
+
+      (* val _ = varname_x |> @{print} *)
+      (* val _ = varname_x1 |> @{print} *)
+
+      val helper_thm = if lr then @{thm index_var_conv_helper1} else  @{thm index_var_conv_helper2}
+  
+      val name_x = varname_x |> Thm.concl_of |> Logic.dest_equals |> snd
+      val name_eq = Raw_Simplifier.rewrite_cterm (false,false,false) (fn _ => fn _ => NONE) ctxt
+        (@{term "op@ :: string=>_=>_"} $ name_x $ HOLogic.mk_string suffix |> Thm.cterm_of ctxt)
+  in
+    helper_thm OF [varname_x, varname_x1, name_eq]
+  end;;
+
+index_var_conv @{context} @{cterm "index_var True var_x"}
+*}
 
 
-lemma "qrhl D [s1,sample x_var Expr[uniform {0..x}] ] [t1,t2,t3] Expr[ Cla[x1\<ge>0] ]"
+ML {*
+  fun index_var_simproc _ ctxt ct = SOME (index_var_conv ctxt ct) handle CTERM _ => NONE
+*}
+
+simproc_setup index_var ("index_var lr v") = index_var_simproc
+
+lemma
+  assumes [simp]: "x\<ge>0"
+  shows "qrhl D [s1,sample var_x Expr[uniform {0..max x 0}] ] [t1,t2,t3] Expr[ Cla[x1\<ge>0] ]"
   using [[method_error]]
   apply (tactic \<open>Tactics.wp1_tac @{context} 1\<close>)
   apply simp
-  oops
+  by (rule qrhl_top)
 
-term a_var
-definition "p1 = [ assign a_var Expr[1], assign b_var Expr[2] ]"
-term a_var
-definition "p2 = [ assign a_var Expr[3], assign b_var Expr[4] ]"
-
-ML {* Tactics.take_n_thm @{context} 2 *}
-
-ML {* Type.constraint *}
-
-lemma lem: "QRHL {Cla[True]} p1 p2 {Cla[True]}"
-  unfolding p1_def p2_def
-  using[[method_error=true]]
-  apply (seq 1 1 "Cla[a1=b1]")
-  sorry
-
-ML {*
-QRHL.VarTypes.get @{context} |> Symtab.dest
-*}
-
-lemma xx[simp]: "1=2" sorry
 
 end
 
-ML {*
-QRHL.VarTypes.get @{context} |> Symtab.dest
-*}
-
+lemma "quantum_equality_full idOp \<lbrakk>q1\<rbrakk> hadamard \<lbrakk>q2\<rbrakk> \<le> (INF (b1, b2):supp (map_distr (\<lambda>b::bit. (b, b + 1)) (uniform UNIV)). 
+case (va, va) of (b1, b2) \<Rightarrow> quantum_equality_full idOp \<lbrakk>q1\<rbrakk> hadamard \<lbrakk>q2\<rbrakk> \<sqinter> \<CC>\<ll>\<aa>[b1 \<noteq> b2])
+"
+  apply simp
 
 end
